Prove Tarjan pending set_fa preservation

SeparationLogic/algorithms/Tarjan_directed/Tarjan_scc_is_low.v
@@ -136,12 +136,26 @@ Section IS_LOW.
     OrderFacts s /\
     (fa s u <> u -> Edge (fa s u) u).
 
+  (* Loop-progress meaning of [done]: every already materialized DFS-tree
+     child of [u] must come from a processed outgoing edge.  The [Visited]
+     guard is intentional: [set_fa child u] may create a pending parent
+     pointer before [child] is visited, and that transient state must not
+     violate the parent loop invariant. *)
+  Definition ProcessedTreeChild
+             (u: V) (done: V -> Prop) (s: St): Prop :=
+    forall child,
+      Visited child s ->
+      fa s child = u ->
+      fa s child <> child ->
+      done child.
+
   Definition LoopCoreShape (u: V) (done: V -> Prop) (s: St): Prop :=
     wf_scc_state g root s /\
     TreeEdgesAreGraphEdges s /\
     Visited u s /\
     (forall a, done a -> Edge u a) /\
-    (forall a, done a -> Visited a s).
+    (forall a, done a -> Visited a s) /\
+    ProcessedTreeChild u done s.
 
   (* Auxiliary facts needed to resume the concrete program frame and to
      run the pop proof.  They are deliberately outside [LoopCoreShape]:
@@ -254,7 +268,7 @@ Section IS_LOW.
     unfold done_after. sets_unfold. auto.
   Qed.
 
-  Lemma PartialTree_done_mono (u a x: V) (done: V -> Prop) (s: St):
+  Lemma partial_tree_done_mono (u a x: V) (done: V -> Prop) (s: St):
     PartialTree u done s x ->
     PartialTree u (done_after done a) s x.
   Proof.
@@ -265,7 +279,7 @@ Section IS_LOW.
       apply done_after_intro_old. exact Hdone.
   Qed.
 
-  Lemma PartialActiveTarget_done_mono
+  Lemma partial_active_target_done_mono
         (u a b: V) (done: V -> Prop) (s: St):
     PartialActiveTarget u done s b ->
     PartialActiveTarget u (done_after done a) s b.
@@ -281,7 +295,7 @@ Section IS_LOW.
       apply done_after_intro_old. exact Hdone.
   Qed.
 
-  Lemma PartialLowCandidate_done_mono
+  Lemma partial_low_candidate_done_mono
         (u a b: V) (done: V -> Prop) (s: St):
     PartialLowCandidate u done s b ->
     PartialLowCandidate u (done_after done a) s b.
@@ -289,22 +303,22 @@ Section IS_LOW.
     intros Ht. unfold PartialLowCandidate in *.
     destruct Ht as [Hb | Hactive].
     - left. exact Hb.
-    - right. apply PartialActiveTarget_done_mono. exact Hactive.
+    - right. apply partial_active_target_done_mono. exact Hactive.
   Qed.
 
-  Lemma PartialTree_root (u: V) (done: V -> Prop) (s: St):
+  Lemma partial_tree_root (u: V) (done: V -> Prop) (s: St):
     PartialTree u done s u.
   Proof.
     unfold PartialTree. left. reflexivity.
   Qed.
 
-  Lemma PartialLowCandidate_root (u: V) (done: V -> Prop) (s: St):
+  Lemma partial_low_candidate_root (u: V) (done: V -> Prop) (s: St):
     PartialLowCandidate u done s u.
   Proof.
     unfold PartialLowCandidate. left. reflexivity.
   Qed.
 
-  Lemma PartialActiveTarget_direct
+  Lemma partial_active_target_direct
         (u a: V) (done: V -> Prop) (s: St):
     Edge u a ->
     Active a s ->
@@ -316,7 +330,7 @@ Section IS_LOW.
     apply done_after_intro_new.
   Qed.
 
-  Lemma PartialLowCandidate_direct_active
+  Lemma partial_low_candidate_direct_active
         (u a: V) (done: V -> Prop) (s: St):
     Edge u a ->
     Active a s ->
@@ -324,16 +338,16 @@ Section IS_LOW.
     PartialLowCandidate u (done_after done a) s a.
   Proof.
     intros Hedge Hactive Hntr.
-    right. apply PartialActiveTarget_direct; auto.
+    right. apply partial_active_target_direct; auto.
   Qed.
 
-  Lemma LowCorrect_empty (u: V) (s: St):
+  Lemma low_correct_empty (u: V) (s: St):
     low s u = dfn s u ->
     LowCorrect u ∅ s.
   Proof.
     intros Hlow. split.
     - exists u. split.
-      + apply PartialLowCandidate_root.
+      + apply partial_low_candidate_root.
       + exact Hlow.
     - unfold LowComplete. intros b Ht.
       unfold PartialLowCandidate in Ht.
@@ -344,14 +358,16 @@ Section IS_LOW.
           sets_unfold in Hdone; tauto.
   Qed.
 
-  Lemma LowComplete_done_mono
+  Lemma low_complete_done_mono
         (u a: V) (done: V -> Prop) (s: St):
     LowComplete u (done_after done a) s ->
     LowComplete u done s.
   Proof.
     unfold LowComplete. intros H b Ht.
-    apply H. apply PartialLowCandidate_done_mono. exact Ht.
+    apply H. apply partial_low_candidate_done_mono. exact Ht.
   Qed.
+
+  (** Preloop **)
 
   Lemma preloop_low_eq_dfn (u: V):
     Hoare (fun _ : St => True)
@@ -433,7 +449,24 @@ Section IS_LOW.
     intros _ s _ w Hempty. sets_unfold in Hempty. tauto.
   Qed.
 
-  Lemma PreloopPreservesClosed (u: V):
+  Lemma preloop_processed_tree_child_empty (u: V):
+    Hoare (fun s: St => wf_scc_state_pre g root u s)
+          (preloop u)
+          (fun _ s => ProcessedTreeChild u ∅ s).
+  Proof.
+    unfold preloop. unfold_op. intro_state. hoare_auto_s.
+    subst s. simpl.
+    destruct H as [[_ [_ [_ Hfa_visited]]] Hunvis].
+    unfold ProcessedTreeChild, Visited.
+    intros child Hchild_vis Hfa Hfane.
+    sets_unfold in Hchild_vis.
+    destruct Hchild_vis as [Hchild_vis_old | Hchild_eq_u].
+    - exfalso. apply Hunvis.
+      rewrite <- Hfa. apply Hfa_visited. exact Hfane.
+    - subst child. exfalso. apply Hfane. exact Hfa.
+  Qed.
+
+  Lemma preloop_preserves_closed (u: V):
     Hoare
       (fun s: St =>
          wf_scc_state_pre g root u s /\
@@ -460,17 +493,17 @@ Section IS_LOW.
     - subst v. apply Hvinact_post. left. reflexivity.
   Qed.
 
-  Lemma PreloopProducesLowCorrectEmpty (u: V):
+  Lemma preloop_produces_low_correct_empty (u: V):
     Hoare (fun _ : St => True)
           (preloop u)
           (fun _ s => LowCorrect u ∅ s).
   Proof.
     eapply Hoare_conseq_post.
     2: apply preloop_low_eq_dfn.
-    intros ret s Hlow. apply LowCorrect_empty. exact Hlow.
+    intros ret s Hlow. apply low_correct_empty. exact Hlow.
   Qed.
 
-  Lemma PreloopProducesLoopCoreShape (u: V):
+  Lemma preloop_produces_loop_core_shape (u: V):
     Hoare (EntryPre u)
           (preloop u)
           (fun _ s => LoopCoreShape u ∅ s).
@@ -497,12 +530,17 @@ Section IS_LOW.
     { eapply Hoare_conseq_pre.
       2: apply preloop_empty_done_edges.
       intros s _. exact I. }
+    apply Hoare_conj with
+      (Q1 := fun _ s => forall a, ∅ a -> Visited a s).
     { eapply Hoare_conseq_pre.
       2: apply preloop_empty_done_visited.
       intros s _. exact I. }
+    { eapply Hoare_conseq_pre.
+      2: apply preloop_processed_tree_child_empty.
+      intros s [Hwf _]. exact Hwf. }
   Qed.
 
-  Lemma PreloopProducesLoopAuxFacts (u: V):
+  Lemma preloop_produces_loop_aux_facts (u: V):
     Hoare (EntryPre u)
           (preloop u)
           (fun _ s => LoopAuxFacts u s).
@@ -542,7 +580,7 @@ Section IS_LOW.
       exact (conj Hnodup (conj Hsiv Hunvis)). }
   Qed.
 
-  Theorem PreloopInitializesLoopInv (u: V):
+  Theorem preloop_initializes_loop_inv (u: V):
     Hoare (EntryPre u)
           (preloop u)
           (fun _ s => LoopInv u ∅ s).
@@ -550,19 +588,499 @@ Section IS_LOW.
     unfold LoopInv, LoopCoreInv.
     apply Hoare_conj with
       (Q1 := fun _ s => LoopAuxFacts u s).
-    { apply PreloopProducesLoopAuxFacts. }
+    { apply preloop_produces_loop_aux_facts. }
     apply Hoare_conj with
       (Q1 := fun _ s => LoopCoreShape u ∅ s).
-    { apply PreloopProducesLoopCoreShape. }
+    { apply preloop_produces_loop_core_shape. }
     apply Hoare_conj with
       (Q1 := fun _ s => Closed s).
     { eapply Hoare_conseq_pre.
-      2: apply PreloopPreservesClosed.
+      2: apply preloop_preserves_closed.
       intros s [Hwf [Hsettled [Hclosed _]]].
       exact (conj Hwf (conj Hsettled Hclosed)). }
     { eapply Hoare_conseq_pre.
-      2: apply PreloopProducesLowCorrectEmpty.
+      2: apply preloop_produces_low_correct_empty.
       intros s _. exact I. }
   Qed.
 
+  (* edge loop *)
+
+  (* 1. state preservation lemmas *)
+
+  Lemma update_low_value (u: V) (n old: nat):
+    Hoare (fun s: St => low s u = old)
+          (update_low u n)
+          (fun _ s => low s u = Nat.min old n).
+  Proof.
+    unfold update_low. unfold_op. intro_state. hoare_auto_s.
+    - subst s. simpl.
+      unfold equiv_decb.
+      destruct (equiv_dec u u) as [_ | Hneq].
+      + rewrite Nat.min_r; lia.
+      + exfalso. apply Hneq. reflexivity.
+    - destruct H as [Heq Hnot_lt]. subst s.
+      rewrite Nat.min_l; lia.
+  Qed.
+
+  Lemma update_low_preserves_closed (u: V) (n: nat):
+    Hoare (Closed)
+          (update_low u n)
+          (fun _ s => Closed s).
+  Proof.
+    unfold update_low. unfold_op. intro_state. hoare_auto_s.
+    - subst s. simpl. exact H.
+    - destruct H1 as [Heq _]. subst s. exact H.
+  Qed.
+
+  Lemma update_low_preserves_tree_edges_are_graph_edges (u: V) (n: nat):
+    Hoare (TreeEdgesAreGraphEdges)
+          (update_low u n)
+          (fun _ s => TreeEdgesAreGraphEdges s).
+  Proof.
+    unfold update_low. unfold_op. intro_state. hoare_auto_s.
+    - subst s. simpl. exact H.
+    - destruct H1 as [Heq _]. subst s. exact H.
+  Qed.
+
+  Lemma update_low_preserves_processed_tree_child
+        (center: V) (done: V -> Prop) (u: V) (n: nat):
+    Hoare (ProcessedTreeChild center done)
+          (update_low u n)
+          (fun _ s => ProcessedTreeChild center done s).
+  Proof.
+    unfold update_low. unfold_op. intro_state. hoare_auto_s.
+    - subst s. simpl. exact H.
+    - destruct H1 as [Heq _]. subst s. exact H.
+  Qed.
+
+  Lemma update_low_preserves_stack_nodup (u: V) (n: nat):
+    Hoare (StackNoDup)
+          (update_low u n)
+          (fun _ s => StackNoDup s).
+  Proof.
+    unfold update_low. unfold_op. intro_state. hoare_auto_s.
+    - subst s. simpl. exact H.
+    - destruct H1 as [Heq _]. subst s. exact H.
+  Qed.
+
+  Lemma update_low_preserves_loop_core_shape
+        (center: V) (done: V -> Prop) (u: V) (n: nat):
+    Hoare
+      (fun s: St => LoopCoreShape center done s /\ u ∈ visited s)
+      (update_low u n)
+      (fun _ s => LoopCoreShape center done s).
+  Proof.
+    unfold LoopCoreShape.
+    unfold update_low. unfold_op. intro_state. hoare_auto_s.
+    - subst s. simpl.
+      destruct H as [[Hwf [Htree [Hvis [Hedge [Hvis_done Hprocessed]]]]] _].
+      split; [exact Hwf |].
+      split.
+      { unfold TreeEdgesAreGraphEdges, tree_edge, Edge in *.
+        simpl. exact Htree. }
+      split; [exact Hvis |].
+      split; [exact Hedge |].
+      split; [exact Hvis_done |].
+      unfold ProcessedTreeChild, Visited in *.
+      simpl. exact Hprocessed.
+    - destruct H1 as [Heq _]. subst s.
+      exact (proj1 H).
+  Qed.
+
+  Lemma update_low_preserves_loop_aux_facts (center u: V) (n: nat):
+    Hoare (LoopAuxFacts center)
+          (update_low u n)
+          (fun _ s => LoopAuxFacts center s).
+  Proof.
+    unfold LoopAuxFacts, OrderFacts.
+    apply Hoare_conj with
+      (Q1 := fun _ s => NoUnvisitedReach s).
+    { eapply Hoare_conseq_pre.
+      2: apply update_low_keep_settled_closed.
+      intros s [Hsettled _]. exact Hsettled. }
+    apply Hoare_conj with
+      (Q1 := fun _ s => Active center s).
+    { eapply Hoare_conseq_pre.
+      2: apply (update_low_keep_in_stack u center n).
+      intros s [_ [Hactive _]]. exact Hactive. }
+    apply Hoare_conj with
+      (Q1 := fun _ s => stack_dfn_order s).
+    { eapply Hoare_conseq_pre.
+      2: apply update_low_keep_stack_dfn_order.
+      intros s [_ [_ [Hstack_order _]]]. exact Hstack_order. }
+    apply Hoare_conj with
+      (Q1 := fun _ s => dfn_injective s).
+    { eapply Hoare_conseq_pre.
+      2: apply update_low_keep_dfn_injective.
+      intros s [_ [_ [_ [Hinj _]]]]. exact Hinj. }
+    { eapply Hoare_conseq_pre.
+      2: apply update_low_preserves_stack_nodup.
+      intros s [_ [_ [_ [_ Hnodup]]]]. exact Hnodup. }
+  Qed.
+
+  Lemma update_low_preserves_loop_inv_shape
+        (center: V) (done: V -> Prop) (u: V) (n: nat):
+    Hoare
+      (fun s: St => LoopInv center done s /\ u ∈ visited s)
+      (update_low u n)
+      (fun _ s =>
+         LoopAuxFacts center s /\
+         LoopCoreShape center done s /\
+         Closed s).
+  Proof.
+    apply Hoare_conj with
+      (Q1 := fun _ s => LoopAuxFacts center s).
+    { eapply Hoare_conseq_pre.
+      2: apply update_low_preserves_loop_aux_facts.
+      intros s [[Haux _] _]. exact Haux. }
+    apply Hoare_conj with
+      (Q1 := fun _ s => LoopCoreShape center done s).
+    { eapply Hoare_conseq_pre.
+      2: apply update_low_preserves_loop_core_shape.
+      intros s [[_ [Hshape _]] Huvis]. exact (conj Hshape Huvis). }
+    { eapply Hoare_conseq_pre.
+      2: apply update_low_preserves_closed.
+      intros s [[_ [_ [Hclosed _]]] _]. exact Hclosed. }
+  Qed.
+
+  Lemma set_fa_state_keep_other_fa (s: St) (v p w: V):
+    w <> v ->
+    fa (set_fa_state s v p) w = fa s w.
+  Proof.
+    intros Hneq.
+    unfold set_fa_state. simpl.
+    unfold equiv_decb.
+    destruct (equiv_dec w v) as [Heq | _].
+    - exfalso. apply Hneq. exact Heq.
+    - reflexivity.
+  Qed.
+
+  Lemma set_fa_pending_tree_step_iff (s: St) (v p x y: V):
+    ~ Visited v s ->
+    (tree_edge (set_fa_state s v p) x y <-> tree_edge s x y).
+  Proof.
+    intros Hnotvis. split.
+    - unfold tree_edge, dg_step.
+      intros [e [Htree [Hfst Hsnd]]].
+      exists e. split; [| split; [exact Hfst | exact Hsnd]].
+      unfold state_to_dfs_tree in Htree |- *. simpl in Htree |- *.
+      destruct Htree as [child [Hchild_vis [Hfane [Hfst_fa Hsnd_child]]]].
+      assert (Hchild_ne: child <> v).
+      { intros Heq. apply Hnotvis. rewrite <- Heq. exact Hchild_vis. }
+      exists child. split; [exact Hchild_vis | split].
+      + unfold equiv_decb in Hfane.
+        destruct (equiv_dec child v) as [Heq | _].
+        * exfalso. apply Hchild_ne. exact Heq.
+        * exact Hfane.
+      + split.
+        * unfold equiv_decb in Hfst_fa.
+          destruct (equiv_dec child v) as [Heq | _].
+          -- exfalso. apply Hchild_ne. exact Heq.
+          -- exact Hfst_fa.
+        * exact Hsnd_child.
+    - unfold tree_edge, dg_step.
+      intros [e [Htree [Hfst Hsnd]]].
+      exists e. split; [| split; [exact Hfst | exact Hsnd]].
+      unfold state_to_dfs_tree in Htree |- *. simpl in Htree |- *.
+      destruct Htree as [child [Hchild_vis [Hfane [Hfst_fa Hsnd_child]]]].
+      assert (Hchild_ne: child <> v).
+      { intros Heq. apply Hnotvis. rewrite <- Heq. exact Hchild_vis. }
+      exists child. split; [exact Hchild_vis | split].
+      + unfold set_fa_state. simpl. unfold equiv_decb.
+        destruct (equiv_dec child v) as [Heq | _].
+        * exfalso. apply Hchild_ne. exact Heq.
+        * exact Hfane.
+      + split.
+        * unfold set_fa_state. simpl. unfold equiv_decb.
+          destruct (equiv_dec child v) as [Heq | _].
+          -- exfalso. apply Hchild_ne. exact Heq.
+          -- exact Hfst_fa.
+        * exact Hsnd_child.
+  Qed.
+
+  Lemma set_fa_pending_tree_reachable_iff (s: St) (v p x y: V):
+    ~ Visited v s ->
+    (dg_reachable (state_to_dfs_tree g (set_fa_state s v p) root) x y <->
+     dg_reachable (state_to_dfs_tree g s root) x y).
+  Proof.
+    intros Hnotvis. split; intro Hreach.
+    - eapply dg_reachable_lift.
+      + intros a b Hstep.
+        apply (proj1 (set_fa_pending_tree_step_iff s v p a b Hnotvis)).
+        exact Hstep.
+      + exact Hreach.
+    - eapply dg_reachable_lift.
+      + intros a b Hstep.
+        apply (proj2 (set_fa_pending_tree_step_iff s v p a b Hnotvis)).
+        exact Hstep.
+      + exact Hreach.
+  Qed.
+
+  Lemma set_fa_pending_preserves_tree_edges_are_graph_edges
+        (s: St) (v p: V):
+    ~ Visited v s ->
+    TreeEdgesAreGraphEdges s ->
+    TreeEdgesAreGraphEdges (set_fa_state s v p).
+  Proof.
+    intros Hnotvis Htree_sound x y Htree.
+    apply Htree_sound.
+    apply (proj1 (set_fa_pending_tree_step_iff s v p x y Hnotvis)).
+    exact Htree.
+  Qed.
+
+  Lemma set_fa_pending_preserves_wf_scc_state (s: St) (u v: V):
+    wf_scc_state g root s ->
+    Visited u s ->
+    ~ Visited v s ->
+    wf_scc_state g root (set_fa_state s v u).
+  Proof.
+    intros [Hstack_vis [Hdfn_inv [Hdfn_valid Hfa_vis]]] Huvis Hnotvis.
+    unfold wf_scc_state. split; [| split; [| split]].
+    - unfold stack_in_visited in *. simpl. exact Hstack_vis.
+    - unfold dfn_inv in *. simpl. exact Hdfn_inv.
+    - unfold dfn_valid in *. simpl.
+      intros x y Hstep.
+      apply Hdfn_valid.
+      apply (proj1 (set_fa_pending_tree_step_iff s v u x y Hnotvis)).
+      exact Hstep.
+    - unfold fa_visited in *. simpl.
+      intros w Hfane.
+      unfold equiv_decb in Hfane |- *.
+      destruct (equiv_dec w v) as [Hw_eq_v | Hw_ne_v].
+      + exact Huvis.
+      + apply Hfa_vis. exact Hfane.
+  Qed.
+
+  Lemma set_fa_pending_preserves_processed_tree_child
+        (center: V) (done: V -> Prop) (s: St) (v p: V):
+    ~ Visited v s ->
+    ProcessedTreeChild center done s ->
+    ProcessedTreeChild center done (set_fa_state s v p).
+  Proof.
+    intros Hnotvis Hprocessed child Hchild_vis Hfa Hfane.
+    simpl in Hchild_vis.
+    assert (Hchild_ne: child <> v).
+    { intros Heq. apply Hnotvis. rewrite <- Heq. exact Hchild_vis. }
+    apply (Hprocessed child Hchild_vis).
+    - rewrite set_fa_state_keep_other_fa in Hfa; auto.
+    - rewrite set_fa_state_keep_other_fa in Hfane; auto.
+  Qed.
+
+  Lemma set_fa_pending_preserves_loop_core_shape
+        (center: V) (done: V -> Prop) (s: St) (v p: V):
+    Visited p s ->
+    ~ Visited v s ->
+    LoopCoreShape center done s ->
+    LoopCoreShape center done (set_fa_state s v p).
+  Proof.
+    intros Hpvis Hnotvis [Hwf [Htree_sound [Hcenter_vis [Hdone_edge [Hdone_vis Hprocessed]]]]].
+    assert (Hwf_post: wf_scc_state g root (set_fa_state s v p)).
+    { apply set_fa_pending_preserves_wf_scc_state; auto. }
+    assert (Htree_post: TreeEdgesAreGraphEdges (set_fa_state s v p)).
+    { apply set_fa_pending_preserves_tree_edges_are_graph_edges; auto. }
+    assert (Hcenter_vis_post: Visited center (set_fa_state s v p)).
+    { simpl. exact Hcenter_vis. }
+    assert (Hdone_vis_post:
+              forall a, done a -> Visited a (set_fa_state s v p)).
+    { intros a Hdone. simpl. apply Hdone_vis. exact Hdone. }
+    assert (Hprocessed_post:
+              ProcessedTreeChild center done (set_fa_state s v p)).
+    { apply set_fa_pending_preserves_processed_tree_child; auto. }
+    exact (conj Hwf_post
+            (conj Htree_post
+              (conj Hcenter_vis_post
+                (conj Hdone_edge
+                  (conj Hdone_vis_post Hprocessed_post))))).
+  Qed.
+
+  Lemma set_fa_pending_partial_active_target_iff
+        (center: V) (done: V -> Prop) (s: St) (v p b: V):
+    ~ Visited v s ->
+    (forall a, done a -> Visited a s) ->
+    (PartialActiveTarget center done (set_fa_state s v p) b <->
+     PartialActiveTarget center done s b).
+  Proof.
+    intros Hnotvis Hdone_vis. split; intro Htarget.
+    - unfold PartialActiveTarget in Htarget |- *.
+      destruct Htarget as [Hdirect | Hchild].
+      + destruct Hdirect as [a [Hdone [Hb [Hedge [Hactive Hnot_tree]]]]].
+        left. exists a.
+        split; [exact Hdone | split; [exact Hb | split; [exact Hedge | split]]].
+        * simpl in Hactive. exact Hactive.
+        * intros Htree.
+          apply Hnot_tree.
+          apply (proj2 (set_fa_pending_tree_step_iff s v p center a Hnotvis)).
+          exact Htree.
+      + destruct Hchild as
+          [child [x [Hdone [Hedge [Hfa [Hfane [Hreach [Hxb [Hactive Hnot_tree]]]]]]]]].
+        assert (Hchild_ne: child <> v).
+        { intros Heq. apply Hnotvis. rewrite <- Heq. apply Hdone_vis. exact Hdone. }
+        right. exists child, x.
+        split; [exact Hdone | split; [exact Hedge | split]].
+        * rewrite set_fa_state_keep_other_fa in Hfa; auto.
+        * split.
+          -- rewrite set_fa_state_keep_other_fa in Hfane; auto.
+          -- split.
+             ++ apply (proj1 (set_fa_pending_tree_reachable_iff s v p child x Hnotvis)).
+                exact Hreach.
+             ++ split; [exact Hxb | split].
+                ** simpl in Hactive. exact Hactive.
+                ** intros Htree.
+                   apply Hnot_tree.
+                   apply (proj2 (set_fa_pending_tree_step_iff s v p x b Hnotvis)).
+                   exact Htree.
+    - unfold PartialActiveTarget in Htarget |- *.
+      destruct Htarget as [Hdirect | Hchild].
+      + destruct Hdirect as [a [Hdone [Hb [Hedge [Hactive Hnot_tree]]]]].
+        left. exists a.
+        split; [exact Hdone | split; [exact Hb | split; [exact Hedge | split]]].
+        * simpl. exact Hactive.
+        * intros Htree.
+          apply Hnot_tree.
+          apply (proj1 (set_fa_pending_tree_step_iff s v p center a Hnotvis)).
+          exact Htree.
+      + destruct Hchild as
+          [child [x [Hdone [Hedge [Hfa [Hfane [Hreach [Hxb [Hactive Hnot_tree]]]]]]]]].
+        assert (Hchild_ne: child <> v).
+        { intros Heq. apply Hnotvis. rewrite <- Heq. apply Hdone_vis. exact Hdone. }
+        right. exists child, x.
+        split; [exact Hdone | split; [exact Hedge | split]].
+        * rewrite set_fa_state_keep_other_fa; auto.
+        * split.
+          -- rewrite set_fa_state_keep_other_fa; auto.
+          -- split.
+             ++ apply (proj2 (set_fa_pending_tree_reachable_iff s v p child x Hnotvis)).
+                exact Hreach.
+             ++ split; [exact Hxb | split].
+                ** simpl. exact Hactive.
+                ** intros Htree.
+                   apply Hnot_tree.
+                   apply (proj1 (set_fa_pending_tree_step_iff s v p x b Hnotvis)).
+                   exact Htree.
+  Qed.
+
+  Lemma set_fa_pending_partial_low_candidate_iff
+        (center: V) (done: V -> Prop) (s: St) (v p b: V):
+    ~ Visited v s ->
+    (forall a, done a -> Visited a s) ->
+    (PartialLowCandidate center done (set_fa_state s v p) b <->
+     PartialLowCandidate center done s b).
+  Proof.
+    intros Hnotvis Hdone_vis.
+    unfold PartialLowCandidate. split; intros [Hb | Htarget].
+    - left. exact Hb.
+    - right.
+      apply (proj1 (set_fa_pending_partial_active_target_iff
+                      center done s v p b Hnotvis Hdone_vis)).
+      exact Htarget.
+    - left. exact Hb.
+    - right.
+      apply (proj2 (set_fa_pending_partial_active_target_iff
+                      center done s v p b Hnotvis Hdone_vis)).
+      exact Htarget.
+  Qed.
+
+  Lemma set_fa_pending_preserves_low_correct
+        (center: V) (done: V -> Prop) (s: St) (v p: V):
+    ~ Visited v s ->
+    (forall a, done a -> Visited a s) ->
+    LowCorrect center done s ->
+    LowCorrect center done (set_fa_state s v p).
+  Proof.
+    intros Hnotvis Hdone_vis [Hsound Hcomplete]. split.
+    - destruct Hsound as [b [Hcandidate Hlow]].
+      exists b. split.
+      + apply (proj2 (set_fa_pending_partial_low_candidate_iff
+                        center done s v p b Hnotvis Hdone_vis)).
+        exact Hcandidate.
+      + simpl. exact Hlow.
+    - intros b Hcandidate.
+      simpl.
+      apply Hcomplete.
+      apply (proj1 (set_fa_pending_partial_low_candidate_iff
+                      center done s v p b Hnotvis Hdone_vis)).
+      exact Hcandidate.
+  Qed.
+
+  Lemma set_fa_pending_preserves_closed (s: St) (v p: V):
+    Closed s ->
+    Closed (set_fa_state s v p).
+  Proof.
+    unfold Closed, Visited, Active.
+    simpl. auto.
+  Qed.
+
+  Lemma set_fa_pending_preserves_loop_core_inv
+        (center: V) (done: V -> Prop) (s: St) (v p: V):
+    Visited p s ->
+    ~ Visited v s ->
+    LoopCoreInv center done s ->
+    LoopCoreInv center done (set_fa_state s v p).
+  Proof.
+    intros Hpvis Hnotvis [Hshape [Hclosed Hlow]].
+    destruct Hshape as [Hwf [Htree_sound [Hcenter_vis [Hdone_edge [Hdone_vis Hprocessed]]]]].
+    assert (Hshape_post: LoopCoreShape center done (set_fa_state s v p)).
+    { apply set_fa_pending_preserves_loop_core_shape; auto.
+      exact (conj Hwf
+              (conj Htree_sound
+                (conj Hcenter_vis
+                  (conj Hdone_edge
+                    (conj Hdone_vis Hprocessed))))). }
+    assert (Hclosed_post: Closed (set_fa_state s v p)).
+    { apply set_fa_pending_preserves_closed. exact Hclosed. }
+    assert (Hlow_post: LowCorrect center done (set_fa_state s v p)).
+    { apply set_fa_pending_preserves_low_correct; auto. }
+    exact (conj Hshape_post (conj Hclosed_post Hlow_post)).
+  Qed.
+
+  Lemma set_fa_pending_preserves_parent_core
+        (u v: V) (done: V -> Prop):
+    Hoare
+      (fun s: St =>
+         LoopCoreInv u done s /\
+         Edge u v /\
+         Active u s /\
+         ~ Visited v s)
+      (set_fa v u)
+      (fun _ s => LoopCoreInv u done s).
+  Proof.
+    unfold set_fa. intro_state. hoare_auto_s.
+    subst s. change (LoopCoreInv u done (set_fa_state s0 v u)).
+    destruct H as [Hcore [_ [_ Hnotvis]]].
+    destruct Hcore as [Hshape [Hclosed Hlow]].
+    destruct Hshape as [Hwf [Htree_sound [Huvis [Hdone_edge [Hdone_vis Hprocessed]]]]].
+    apply set_fa_pending_preserves_loop_core_inv; auto.
+    exact (conj
+             (conj Hwf
+               (conj Htree_sound
+                 (conj Huvis
+                   (conj Hdone_edge
+                     (conj Hdone_vis Hprocessed)))))
+             (conj Hclosed Hlow)).
+  Qed.
+
+  Lemma current_active_edge_not_tree
+        (u v: V) (done: V -> Prop) (s: St):
+    LoopInv u done s ->
+    Edge u v ->
+    ~ done v ->
+    Visited v s ->
+    Active v s ->
+    ~ tree_edge s u v.
+  Proof.
+    intros Hinv _ Hnot_done _ _ Htree.
+    destruct Hinv as [_ [Hshape _]].
+    destruct Hshape as [_ [_ [_ [_ [_ Hprocessed]]]]].
+    unfold tree_edge, dg_step in Htree.
+    destruct Htree as [e [Htree_edge [Hfst Hsnd]]].
+    simpl in Hfst, Hsnd.
+    unfold state_to_dfs_tree in Htree_edge. simpl in Htree_edge.
+    destruct Htree_edge as [child [Hchild_vis [Hfane [Hfst_fa Hsnd_child]]]].
+    assert (Hfa_child: fa s child = u).
+    { rewrite <- Hfst_fa. exact Hfst. }
+    apply Hnot_done.
+    rewrite <- Hsnd.
+    rewrite Hsnd_child.
+    exact (Hprocessed child Hchild_vis Hfa_child Hfane).
+  Qed.
 End IS_LOW.
